Benchmark.lean
@@ -14,8 +14,7 @@ instance : MonadLift (Except String) IO where
     | Except.error e => throw $ .userError e
 
 private def stack_ops (stack : Stack 1 "") : Nat × Stack 1 "" :=
-  let frameStep : Frame 1 "" := Frame.Step default
-                                  (CharPos.create "" (instSubstringValid "").default (by decide))
+  let frameStep : Frame 1 "" := Frame.Step default (CharPos.create "" ⟨0, by simp⟩)
   let frameRestoreCapture : Frame 1 "" := Frame.RestoreCapture Capture.Role.Start default default
   let stack := Stack.push stack frameStep
   let stack := Stack.push stack frameRestoreCapture
@@ -58,7 +57,7 @@ def main (args : List String): IO Unit := do
           let nl := "\n"
 
           let regex ← build re default default ⟨true, false⟩
-          match Regex.Log.captures haystack regex (instSubstringValid haystack).default (logEnabled := false) with
+          match Regex.Log.captures haystack regex default (logEnabled := false) with
           | (msgs, none) =>
             if msgs.size > 0 then IO.println s!"msgs {msgs |> Array.map (· ++ nl)}"
             IO.println s!"captures: none"
