Regex/Basic.lean
@@ -1,4 +1,5 @@
 import Batteries.Data.String
+import Regex.Data.String.Basic
 
 namespace Regex
 
@@ -9,41 +10,23 @@ Definitions for Regex api
 
 -/
 
-abbrev ValidSubstring := { s : Substring // Substring.Valid s }
-abbrev ValidPos s := { pos : String.Pos.Raw // String.Pos.Raw.Valid s pos }
-
-instance instSubstringValid (s : ValidSubstring) : Inhabited (ValidPos s.val.str) where
-  default := ⟨s.val.startPos, s.property.startValid⟩
-
-instance : Coe String ValidSubstring where
-  coe s := ⟨s.toSubstring, String.valid_toSubstring s⟩
+instance : Coe String String.Slice where
+  coe s := s.toSlice
 
 /-- Represents a single match of a regex in a haystack. -/
-abbrev Match := ValidSubstring
+abbrev Match := String.Slice
 
 instance : ToString Match where
   toString s :=
-    s!"'{s}', {s.val.startPos}, {s.val.stopPos}"
+    s!"'{s.copy}', {s.startInclusive.offset}, {s.endExclusive.offset}"
 
 /-- Represents the full match and capture groups for a single match in `s`. -/
-structure Captures (s : String) where
+structure Captures (s : String.Slice) where
   /-- the full match -/
   fullMatch : Match
   /-- the capture groups, empty groups can arise, for example, in alternatives -/
   groups: Array (Option Match)
-  /-- `fullMatch` is a substring of `s`. -/
-  isSubstringOf : fullMatch.val.str = s
-  /-- all matches in `groups` are substrings of `s`. -/
-  areSubstringsOf : groups.all (Option.all (·.val.str = s) ·)
-
-theorem start_pos_valid_of {s : ValidSubstring} (captures : Captures s.val.str)
-    : String.Pos.Raw.Valid s.val.str captures.fullMatch.val.startPos  := by
-  have : captures.fullMatch.val.str = s.val.str := by simp [captures.isSubstringOf]
-  have := captures.fullMatch.property.startValid
-  simp_all
-
-theorem stop_pos_valid_of {s : ValidSubstring} (captures : Captures s.val.str)
-    : String.Pos.Raw.Valid s.val.str captures.fullMatch.val.stopPos  := by
-  have : captures.fullMatch.val.str = s.val.str := by simp [captures.isSubstringOf]
-  have := captures.fullMatch.property.stopValid
-  simp_all
+  /-- `fullMatch` is a subslice of `s`. -/
+  isSubsliceOf : String.Slice.isSubslice fullMatch s
+  /-- all matches in `groups` are subslices of `s`. -/
+  areSubslicesOf : ∀ g ∈ groups.filterMap id, String.Slice.isSubslice g s
