Regex/Data/String/Basic.lean
@@ -1,0 +1,84 @@
+import Batteries.Data.String
+
+namespace String.Slice
+
+/-- Slice `s` is a subslice of Slice `t`, if the underlying strings are equal
+  and t.startInclusive ≤ s.startInclusive and s.endExclusive ≤ t.endExclusive.  -/
+def isSubslice (s t : String.Slice) := s.str = t.str
+                  ∧ t.startInclusive.offset ≤ s.startInclusive.offset
+                  ∧ s.endExclusive.offset ≤ t.endExclusive.offset
+
+@[simp] theorem replaceStartEnd_is_subslice_of {s : String.Slice} {p0 p1 : s.Pos} {h : p0 ≤ p1}
+    : isSubslice (String.Slice.replaceStartEnd s p0 p1 h) s := by
+  and_intros
+  · rfl
+  · simp [String.Pos.Raw.offsetBy, String.Pos.Raw.le_iff]
+  · rw [@String.Slice.endExclusive_replaceStartEnd s p0 p1 h]
+    exact String.Slice.Pos.offset_str_le_offset_endExclusive
+
+/-- cast `p : s.Pos` to `t.Pos` -/
+def castPosOfSubslice {s t : String.Slice} (p: s.Pos) (h : isSubslice s t) : t.Pos :=
+  ⟨⟨p.offset.byteIdx + s.startInclusive.offset.byteIdx - t.startInclusive.offset.byteIdx⟩, by
+    simp [isSubslice] at h
+    generalize heq : p.offset.byteIdx + s.startInclusive.offset.byteIdx - t.startInclusive.offset.byteIdx = byteIdx
+    have le : ⟨byteIdx⟩ ≤ t.rawEndPos := by
+      rw [← heq]
+      simp [String.Slice.rawEndPos, String.Slice.utf8ByteSize_eq]
+
+      have := t.startInclusive_le_endExclusive
+      rw [String.ValidPos.le_iff, String.Pos.Raw.le_iff] at this
+      simp_all only [Nat.sub_add_cancel]
+
+      have := p.isValidForSlice.le_utf8ByteSize
+      simp [Slice.rawEndPos, Slice.utf8ByteSize, Pos.Raw.byteDistance, String.Pos.Raw.le_iff] at this
+
+      have := s.startInclusive_le_endExclusive
+      simp [String.ValidPos.le_iff, String.Pos.Raw.le_iff] at this
+
+      exact Nat.le_trans (by grind) h.right.right
+    have isValid : ((⟨byteIdx⟩ : String.Pos.Raw).offsetBy t.startInclusive.offset).IsValid t.str := by
+      rw [← heq]
+      simp [String.Pos.Raw.offsetBy]
+      rw [Nat.add_sub_cancel' (by have := String.Pos.Raw.le_iff.mp h.right.left; grind)]
+      rw [← h.left]
+      have := p.isValidForSlice.isValid_offsetBy
+      simp [Pos.Raw.offsetBy] at this
+      grind
+    exact { le_utf8ByteSize := le, isValid_offsetBy := isValid }⟩
+
+/-- `s.startPos : s.Pos` as `t.Pos` -/
+def startPosOfSubslice {s t : String.Slice} (h : isSubslice s t) : t.Pos :=
+  castPosOfSubslice s.startPos h
+
+theorem startPosOfSubslice_eq {s t : String.Slice} (h : isSubslice s t)
+    : ⟨s.startInclusive.offset.byteIdx - t.startInclusive.offset.byteIdx⟩
+      = (startPosOfSubslice h).offset := by
+  simp [castPosOfSubslice, startPosOfSubslice]
+
+/-- `s.endPos : s.Pos` as `t.Pos` -/
+def endPosOfSubslice {s t : String.Slice} (h : isSubslice s t) : t.Pos :=
+  castPosOfSubslice s.endPos h
+
+theorem endPosOfSubslice_eq {s t : String.Slice} (h : isSubslice s t)
+    : ⟨s.endExclusive.offset.byteIdx - t.startInclusive.offset.byteIdx⟩
+      = (endPosOfSubslice h).offset := by
+  simp [castPosOfSubslice, endPosOfSubslice]
+  have : s.startInclusive.offset.byteIdx + s.utf8ByteSize = s.endExclusive.offset.byteIdx := by
+    exact Nat.add_sub_of_le s.startInclusive_le_endExclusive
+  grind
+
+@[simp] theorem byteDistance_of_next_lt {s : String.Slice} {pos : s.Pos} (h : pos ≠ s.endPos)
+    : (pos.next h).offset.byteDistance s.rawEndPos < pos.offset.byteDistance s.rawEndPos := by
+  simp [String.Pos.Raw.byteDistance]
+  rw [← @String.Slice.Pos.byteIdx_offset_next s pos h]
+  have : pos.offset.byteIdx < (pos.next h).offset.byteIdx := by
+    have := @String.Slice.Pos.lt_next s pos h
+    rwa [String.Slice.Pos.lt_iff, String.Pos.Raw.lt_iff] at this
+  have : (pos.next h).offset.byteIdx ≤ s.utf8ByteSize :=
+    (pos.next h).isValidForSlice.le_utf8ByteSize
+  grind
+
+@[simp] theorem byteDistance_of_offset_and_char_lt {s : String.Slice} {pos : s.Pos} (h : pos ≠ s.endPos)
+    : (pos.offset + pos.get h).byteDistance s.rawEndPos < pos.offset.byteDistance s.rawEndPos := by
+  rw [← @String.Slice.Pos.offset_next s pos h]
+  exact byteDistance_of_next_lt h
