test/Test.lean
@@ -14,23 +14,23 @@ open Lean System
 
 open Regex
 
-def testToml (path : FilePath) (filename : String) (flavor : Syntax.Flavor) (tests : Array RegexTest)
+def testToml (path : FilePath) (filename : String) (verbose : Bool) (flavor : Syntax.Flavor) (tests : Array RegexTest)
     : IO (Nat × Nat × Nat) := do
-  let (succeeds, failures, ignored) ← RegexTest.testItems flavor filename tests
+  let (succeeds, failures, ignored) ← RegexTest.testItems verbose flavor filename tests
   IO.println s!"succeeds {succeeds} failures {failures} ignored {ignored} in file {path}"
   pure (succeeds, failures, ignored)
 
-def testRustFile (path : FilePath) : IO (Nat × Nat × Nat) := do
+def testRustFile (path : FilePath) (verbose : Bool) : IO (Nat × Nat × Nat) := do
   let filename : String := path.fileName.getD ""
   if #["no-unicode.toml", "regex-lite.toml", "utf8.toml"].contains filename
   then pure (0, 0, 0) else
   let tests ← Loader.Toml.load path
-  testToml path filename Syntax.Flavor.Rust tests
+  testToml path filename verbose Syntax.Flavor.Rust tests
 
-def testPcreFile (path : FilePath) : IO (Nat × Nat × Nat) := do
+def testPcreFile (path : FilePath) (verbose : Bool) : IO (Nat × Nat × Nat) := do
   let filename : String := path.fileName.getD ""
   let tests ← (← Loader.Pcre.load path) |> Loader.Pcre.toRegexTestArray |> IO.ofExcept
-  testToml path filename Syntax.Flavor.Pcre (tests)
+  testToml path filename verbose Syntax.Flavor.Pcre (tests)
 
 def summary (arr : Array (Nat × Nat × Nat)) : IO UInt32 := do
   let (succeeds, failures, ignored) := arr |> Array.foldl
@@ -39,20 +39,20 @@ def summary (arr : Array (Nat × Nat × Nat)) : IO UInt32 := do
   if failures > 0 then IO.eprintln s!"succeeds {succeeds} failures {failures} ignored {ignored} total"
   pure (if failures > 0 then 1 else 0)
 
-def testRustFlavor (path : FilePath) : IO UInt32 := do
+def testRustFlavor (path : FilePath) (verbose : Bool) : IO UInt32 := do
   if ← System.FilePath.isDir path
   then
     (← System.FilePath.walkDir path)
     |> Array.filter (fun f => f.toString.endsWith "toml")
-    |> Array.mapM (fun file => testRustFile file)
+    |> Array.mapM (fun file => testRustFile file verbose)
     |> fun arr => do summary (← arr)
   else
     IO.println  s!"no such directory '{path}'"
     pure 1
 
-def testAllFlavors : IO UInt32 := do
-  let retRust ← testRustFlavor "testdata/rust"
-  let retPcre ← summary #[← testPcreFile "testdata/pcre/testresult1.json"]
+def testAllFlavors (verbose : Bool) : IO UInt32 := do
+  let retRust ← testRustFlavor "testdata/rust" verbose
+  let retPcre ← summary #[← testPcreFile "testdata/pcre/testresult1.json" verbose]
 
   pure (if 0 < retRust + retPcre then 1 else 0)
 
@@ -60,12 +60,14 @@ def main (args : List String): IO UInt32 := do
   let exitcode ←
     try
       match args with
-      | [] => pure <| ← testAllFlavors
-      | ["--pcre", path] => pure <| ← summary #[← testPcreFile path]
-      | ["--toml", path] => pure <| ← summary #[← testRustFile path]
-      | ["--all", path] => pure <| ← testRustFlavor path
+      | [] => pure <| ← testAllFlavors false
+      | ["--pcre", path] => pure <| ← summary #[← testPcreFile path false]
+      | ["--toml", path] => pure <| ← summary #[← testRustFile path false]
+      | ["--toml", path, "-a"] => pure <| ← testRustFlavor path false
+      | ["--toml", path, "-a", "-v"] => pure <| ← testRustFlavor path true
+      | ["--pcre", path, "-v"] => pure <| ←  summary #[← testPcreFile path true]
       | _ =>
-        IO.println  s!"usage: Test [--toml <path> | --pcre] [--all path]"
+        IO.println  s!"usage: Test [--toml <path> |--pcre <path>] [-a] [-v]"
         pure 1
     catch e =>
       IO.println s!"Error: {e}"
